user 3, session 2698, part 3

diffs-annotated/3/user-3-session-2698.v
@@ -69,50 +69,58 @@ Definition bounded0 : {x | x < 256}.
 exists 0.
 (apply Nat.lt_0_succ).
 Defined.
-Definition nat64_to_le (x : nat) : option (list {x | x < 256}) :=
-  let digits := nat_to_le 254 x in
-  if nat_le_dec (length digits) 8
-  then Some (digits ++ repeat bounded0 (8 - length digits))
-  else None.
-Redirect "/var/folders/5x/1mdbpbjd7012l971fq0zkj2w0000gn/T/coq3PKT1A"
+Definition nat64_from_le (digits : list {x | x < 256}) : nat :=
+  nat_from_le digits.
+Redirect "/var/folders/5x/1mdbpbjd7012l971fq0zkj2w0000gn/T/coqIQarSZ"
 Print Ltac Signatures.
 Timeout 1 Print Grammar tactic.
 Add Search Blacklist "Raw" "Proofs".
 Set Search Output Name Only.
-Redirect "/var/folders/5x/1mdbpbjd7012l971fq0zkj2w0000gn/T/coqmyolBc"
-SearchPattern _.
-Remove Search Blacklist "Raw" "Proofs".
-Unset Search Output Name Only.
-Theorem nat_from_le_zeros base_m2 digits zero_v n :
-  proj1_sig zero_v = 0 ->
-  @nat_from_le base_m2 (digits ++ repeat zero_v n) =
-  @nat_from_le base_m2 digits.
-Proof.
-(intros).
-(induction digits; simpl; auto).
-(induction n; simpl; auto).
-lia.
-Qed.
-Definition nat64_from_le (digits : list {x | x < 256}) : 
-  option nat :=
-  if nat_eq_dec (length digits) 8 then Some (nat_from_le digits) else None.
-Redirect "/var/folders/5x/1mdbpbjd7012l971fq0zkj2w0000gn/T/coq2AL3Dg"
-Print Ltac Signatures.
-Timeout 1 Print Grammar tactic.
-Add Search Blacklist "Raw" "Proofs".
-Set Search Output Name Only.
-Redirect "/var/folders/5x/1mdbpbjd7012l971fq0zkj2w0000gn/T/coqWpS2bI"
+Redirect "/var/folders/5x/1mdbpbjd7012l971fq0zkj2w0000gn/T/coqGiBzRk"
 SearchPattern _.
 Remove Search Blacklist "Raw" "Proofs".
 Unset Search Output Name Only.
 Definition bounded_to_ascii (x : {x | x < 256}) : Ascii.ascii :=
   Ascii.ascii_of_nat (proj1_sig x).
-Redirect "/var/folders/5x/1mdbpbjd7012l971fq0zkj2w0000gn/T/coqulyt9M"
-Print Ltac Signatures.
-Timeout 1 Print Grammar tactic.
-Add Search Blacklist "Raw" "Proofs".
-Set Search Output Name Only.
-Redirect "/var/folders/5x/1mdbpbjd7012l971fq0zkj2w0000gn/T/coqt9Zf90"
-SearchPattern _.
-Remove Search Blacklist "Raw" "Proofs".
-Unset Search Output Name Only.
+Definition ascii_to_bounded (a : Ascii.ascii) : {x | x < 256}.
+refine (exist _ (Ascii.nat_of_ascii a) _).
+(apply Ascii.nat_ascii_bounded).
+Defined.
+Instance aModel : GoModel.
+Proof.
+refine
+ {|
+ byte := {x | x < 256};
+ byte0 := exist _ 0 _;
+ uint64_to_string := pretty.pretty_nat;
+ ascii_to_byte := ascii_to_bounded;
+ byte_to_ascii := bounded_to_ascii;
+ uint64_to_le := nat64_to_le;
+ uint64_from_le := nat64_from_le;
+ File := Z;
+ nilFile := (- 1)%Z;
+ Ptr := fun _ => nat;
+ nullptr := fun _ => 0 |}.
+(apply Nat.lt_0_succ).
+Defined.
+Instance aModel_wf : (GoModelWf aModel).
+Proof.
+econstructor.
+-
+(simpl).
+(apply pretty.pretty_nat_inj).
+-
+(simpl).
+(unfold bounded_to_ascii, ascii_to_bounded).
+(intros).
+(destruct c; simpl).
+(rewrite Ascii.ascii_nat_embedding; auto).
+-
+(simpl).
+(destruct b; simpl).
+(unfold ascii_to_bounded, bounded_to_ascii; simpl).
+(apply ProofIrrelevanceTheory.subset_eq_compat).
+(rewrite Ascii.nat_ascii_embedding; auto).
+-
+constructor.
+(intros).
